theories/vir/bij_laws.v
@@ -5,7 +5,8 @@ From iris.prelude Require Import options.
 
 From velliris.base_logic Require Export gen_sim_prog.
 From velliris.program_logic Require Import program_logic.
-From velliris.vir Require Export vir vir_state spec primitive_laws.
+From velliris.vir Require Export
+  vir vir_state spec primitive_laws vir_sim_properties.
 
 From ITree Require Import
   ITree Eq.Eqit Eq.EqAxiom Events.State Events.StateFacts Extra.IForest.
