theories/vir/primitive_laws.v
@@ -11,13 +11,6 @@ From Vellvm Require Import Semantics.LLVMEvents Handlers.Handlers Handlers.Memor
 Set Default Proof Using "Type*".
 
 
-(* TODO: Move *)
-Lemma non_void_allocate_abs:
-  forall τ σ s, non_void τ -> ~ (allocate σ τ = inl s).
-Proof.
-  intros; destruct τ; eauto.
-Qed.
-
 Section proof.
 
   Context {Σ} `{!vellirisGS Σ}.
