theories/vir/tactics.v
@@ -63,3 +63,70 @@ Ltac to_inner G :=
         | SOURCE_EXC => source_exc
         end)%I with
         (sim_expr_inner G (sim_indF G) Φ x y).
+
+
+(* Some useful tactics for reducing [sim_expr] for [vir] *)
+From velliris.vir Require Import vir vir_sim_properties.
+
+Ltac itree_vsimp e :=
+  lazymatch e with
+  (* Conversion lemmas *)
+  | exp_conv (Ret _) => rewrite exp_conv_ret
+  | exp_conv (bind _ _) => rewrite exp_conv_bind
+  | exp_conv (ITree.bind _ _) => rewrite exp_conv_bind
+  | instr_conv (trigger (Call _ _ _ _)) =>
+      rewrite instr_conv_call
+  | instr_conv (trigger _) =>
+      rewrite instr_conv_noncall +
+      rewrite instr_conv_noncall'
+  | instr_conv (Ret ?x) => rewrite (instr_conv_ret x)
+  | instr_conv (Ret _) => rewrite instr_conv_ret
+  | instr_conv (bind _ _) => rewrite instr_conv_bind
+  | instr_conv (ITree.bind _ _) => rewrite instr_conv_bind
+  | L0'expr_conv (Ret _) => rewrite L0'expr_conv_ret
+  | L0'expr_conv (bind _ _) => rewrite L0'expr_conv_bind
+  | L0'expr_conv (ITree.bind _ _) => rewrite L0'expr_conv_bind
+
+  (* Specific to level translations *)
+  | interp (λ T e, Vis (instrE_conv T (exp_to_instr e)) (λ x : T , Ret x)) _ =>
+      rewrite (eq_itree_interp _ _ eq2_exp_to_L0); last done
+ end.
+
+Ltac sim_expr_vsimp e :=
+  match e with
+  (* Event translation adjustment *)
+  | sim_expr _ (L0'expr_conv (translate instr_to_L0' _))
+              (L0'expr_conv (translate instr_to_L0' _)) =>
+      iApply instr_to_L0'
+  | sim_expr _ (instr_conv (translate exp_to_instr _))
+              (instr_conv (translate exp_to_instr _)) =>
+      iApply exp_conv_to_instr
+  (* Vis to [trigger] *)
+  | sim_expr _ (Vis _ _) (Vis _ _ ) =>
+      iApply sim_expr_vis
+  | sim_expr _ (vis _ _) (vis _ _ ) =>
+      iApply sim_expr_vis
+  (* Some symbolic execution under ITree rewrites *)
+  | sim_expr _ ?l ?r =>
+    (* Try doing ITree rewriting on both sides if possible *)
+    (itree_vsimp l + itree_simp l) +
+    (itree_vsimp r + itree_simp r)
+  end.
+
+Ltac vsimp := repeat
+  lazymatch goal with
+  | |- environments.envs_entails _ (bupd ?e) =>
+      iModIntro
+  | |- environments.envs_entails _ ?e =>
+      sim_expr_vsimp e
+  end.
+
+Ltac final :=
+  vsimp;
+  repeat Tau;
+  match goal with
+  (* Base case *)
+  | |- environments.envs_entails _
+      (sim_expr _ (Ret _) (Ret _)) =>
+      iApply sim_expr_base
+  end.
